# Equation_Solver

# SOLVE FOR FOLLOWING 12 UNKNOWNS

Let the unknowns be:

x₁, y₁, x₂, y₂, x₃, y₃, x₄, y₄, x₅, y₅, x₆, y₆ and r

where α, β, ε and z are **known quantities**.

---

## GIVEN EQUATIONS

**EQ‑1**
[ x_4^2 + y_4^2 = z^2 ]

**EQ‑2**
[ (x_5 - x_4)^2 + (y_5 - y_4)^2 = x_1^2 + y_1^2 ]

**EQ‑3**
[ (x_3 - x_2)^2 + (y_3 - y_2)^2 = r^2 ]

**EQ‑4**
[ (x_5 - x_2)^2 + (y_5 - y_2)^2 = r^2 ]

**EQ‑5**
[ (x_6 - x_2)^2 + (y_6 - y_2)^2 = r^2 ]

**EQ‑6**
[ (x_2 - x_1)^2 + (y_2 - y_1)^2 + (x_5 - x_2)^2 + (y_5 - y_2)^2 = z^2 ]

**EQ‑7**
[
(x_6 - x_1)^2 + (y_6 - y_1)^2 = (x_6 - x_2)^2 + (y_6 - y_2)^2 + (x_2 - x_1)^2 + (y_2 - y_1)^2 \

* 2\sqrt{[(x_6 - x_2)^2 + (y_6 - y_2)^2][(x_2 - x_1)^2 + (y_2 - y_1)^2]}\cos\beta
  ]

**EQ‑8**
[
(x_6 - x_5)^2 + (y_6 - y_5)^2 = (x_6 - x_2)^2 + (y_6 - y_2)^2 + (x_5 - x_2)^2 + (y_5 - y_2)^2 \

* 2\sqrt{[(x_6 - x_2)^2 + (y_6 - y_2)^2][(x_5 - x_2)^2 + (y_5 - y_2)^2]}\cos\beta
  ]

**EQ‑9**
[
(x_5 - x_3)^2 + (y_5 - y_3)^2 = (x_5 - x_2)^2 + (y_5 - y_2)^2 + (x_3 - x_2)^2 + (y_3 - y_2)^2 \

* 2\sqrt{[(x_5 - x_2)^2 + (y_5 - y_2)^2][(x_3 - x_2)^2 + (y_3 - y_2)^2]}\cos\varepsilon
  ]

**EQ‑10**
[
(x_6 - x_3)^2 + (y_6 - y_3)^2 = (x_6 - x_2)^2 + (y_6 - y_2)^2 + (x_3 - x_2)^2 + (y_3 - y_2)^2 \

* 2\sqrt{[(x_6 - x_2)^2 + (y_6 - y_2)^2][(x_3 - x_2)^2 + (y_3 - y_2)^2]}\cos(\beta + \varepsilon)
  ]

**EQ‑11**
[
(x_3 - x_1)^2 + (y_3 - y_1)^2 = (x_3 - x_2)^2 + (y_3 - y_2)^2 + (x_2 - x_1)^2 + (y_2 - y_1)^2 \

* 2\sqrt{[(x_3 - x_2)^2 + (y_3 - y_2)^2][(x_2 - x_1)^2 + (y_2 - y_1)^2]}\cos\varepsilon
  ]

**EQ‑12**
[
(x_5 - x_3)^2 + (y_5 - y_3)^2 = (x_4 - x_3)^2 + (y_4 - y_3)^2 + (x_5 - x_4)^2 + (y_5 - y_4)^2 \

* 2\sqrt{[(x_4 - x_3)^2 + (y_4 - y_3)^2][(x_5 - x_4)^2 + (y_5 - y_4)^2]}\cos\alpha
  ]

**EQ‑13**
[ x_2^2 + y_2^2 = (x_2 - x_1)^2 + (y_2 - y_1)^2 + (x_1^2 + y_1^2) ]

---

## CHECK

Given distance:

Distance (|ab| = 0.1943)

[
\sqrt{(x_4 - x_3)^2 + (y_4 - y_3)^2} = 0.1943
]

---

**This version is clean, structured, fully editable, and ideal for direct copy–paste into Word, Google Docs, or LaTeX.**
